cogent/llvm/checker/coq/Denote.v
@@ -1,8 +1,10 @@
 From Coq Require Import List ZArith String.
 
-From ExtLib Require Import Structures.Monads Structures.Functor Structures.Reducible Data.Map.FMapAList.
-From ITree Require Import ITree Events.State Events.Exception Events.FailFacts.
-From Vellvm Require Import Util Utils.Error.
+From ExtLib Require Import Structures.Monads Structures.Functor Structures.Reducible
+  Data.Map.FMapAList.
+From ITree Require Import ITree Events.State Events.Exception Events.FailFacts Events.StateFacts
+  Interp.TranslateFacts Eq.Eq.
+From Vellvm Require Import Util Utils.Error Utils.NoFailure Utils.PropT.
 
 From Checker Require Import Cogent Utils.Instances.
 
@@ -196,16 +198,6 @@ Section Interpretation.
 
 End Interpretation.
 
-Require Export ITree.Interp.TranslateFacts.
-Require Export ITree.Basics.CategoryFacts.
-Require Export ITree.Events.State.
-Require Export ITree.Events.StateFacts.
-Require Export ITree.ITree.
-Require Export ITree.Eq.Eq.
-Require Export ITree.Basics.Basics.
-Require Export ITree.Events.Exception.
-Require Export ITree.Interp.InterpFacts.
-
 Local Open Scope itree_scope.
 
 Section InterpTheory.
@@ -227,6 +219,15 @@ Section InterpTheory.
     intros; unfold interp_mem.
     rewrite interp_state_bind.
     apply eutt_eq_bind; intros []; reflexivity.
+  Qed.
+
+  Lemma interp_Mem_vis_eqit :
+    forall T R mem (e : CogentL0 T) (k : T -> itree CogentL0 R),
+      interp_mem (vis e k) mem ≅ ITree.bind ((case_ handle_mem pure_state) T e mem) (fun sx => Tau (interp_mem (k (snd sx)) (fst sx))).
+  Proof.
+    intros T R mem e k.
+    unfold interp_mem.
+    apply interp_state_vis.
   Qed.
 
   Lemma interp_expr_Ret :
@@ -258,5 +259,61 @@ Section InterpTheory.
     rewrite translate_ret; reflexivity.
   Qed.
 
-
 End InterpTheory.
+
+Section NoFailure.
+
+  Lemma no_failure_expr_Ret : forall E x m,
+    no_failure (interp_expr (E := E) (Ret x) m).
+  Proof.
+    intros.
+    rewrite interp_expr_Ret. apply eutt_Ret; intros abs; inv abs.
+  Qed.
+
+  Lemma failure_expr_throw : forall E s m,
+    ~ no_failure (interp_expr (E := E) (throw s) m).
+  Proof.
+    intros * abs.
+    unfold Exception.throw in *.
+    unfold interp_expr in *.
+    setoid_rewrite interp_Mem_vis_eqit in abs.
+    unfold pure_state in *; cbn in *.
+    rewrite interp_fail_bind in abs.
+    rewrite interp_fail_vis in abs.
+    cbn in *.
+    rewrite Eq.bind_bind, !bind_ret_l in abs.
+    rewrite translate_ret in abs.
+    eapply eutt_Ret in abs.
+    apply abs; auto.
+  Qed.
+
+  Lemma failure_expr_throw' : forall E s (k : uval -> _) m,
+    ~ no_failure (interp_expr (E := E) (ITree.bind (throw s) k) m).
+  Proof.
+    intros * abs.
+    rewrite interp_expr_bind in abs.
+    eapply no_failure_bind_prefix, failure_expr_throw in abs; auto.
+  Qed.
+
+  Lemma no_failure_expr_bind_prefix : forall {E} (t : itree _ uval) (k : uval -> itree _ uval) m,
+    no_failure (interp_expr (E := E) (ITree.bind t k) m) ->
+    no_failure (interp_expr (E := E) t m).
+  Proof.
+    intros * NOFAIL.
+    rewrite interp_expr_bind in NOFAIL.
+    eapply no_failure_bind_prefix; eapply NOFAIL.
+  Qed.
+  
+  Lemma no_failure_expr_bind_continuation :
+    forall {E} (t : itree _ uval) (k : uval -> itree _ uval) m,
+      no_failure (interp_expr (E := E) (ITree.bind t k) m) ->
+      forall u m', Returns (E := E) (Some (m',u)) (interp_expr t m) -> 
+        no_failure (interp_expr (E := E) (k u) m').
+  Proof.
+    intros * NOFAIL * ISRET.
+    rewrite interp_expr_bind in NOFAIL.
+    eapply no_failure_bind_cont in NOFAIL; eauto.
+    apply NOFAIL.
+  Qed.
+
+End NoFailure.
